formal/coq/extraction/TransitionExtraction.v
@@ -65,5 +65,11 @@ Definition extract_valid_block_structural := valid_block_structural.
 Definition extract_apply_block_transitions_structural := apply_block_transitions_structural.
 Definition extract_apply_valid_block_structural := apply_valid_block_structural.
 Definition extract_option_is_some {A : Type} := @option_is_some A.
+Definition extract_utxo_domain := utxo_domain.
+Definition extract_domain_has_no_duplicates := domain_has_no_duplicates.
+Definition extract_domain_below_bool := domain_below_bool.
+Definition extract_block_output_count := block_output_count.
+Definition extract_block_input_outpoints := block_input_outpoints.
+Definition extract_spent_inputs_absent_bool := spent_inputs_absent_bool.
 
 End TransitionExtraction.
